src/tools/parallelcomposition/parallelcompositionsimpleScript.sml
@@ -64,7 +64,7 @@ Define`
 *)
 
 (* multi transitions relation *)
-val _ = Parse.type_abbrev("mtrel", ``:(('symb set) # ('pred set) # 'state) -> ('event list) -> (('symb set) # ('pred set) # 'state) -> bool``);
+val _ = Parse.type_abbrev("mtrel", ``:(('symb set) # ('pred set) # 'state) -> ('event list) -> (('symb set) # ('pred set) # 'state)``);
 
 (* multi transitions system *)    
 val _ = Parse.type_abbrev("multransys", ``:(( 'symb, 'pred, 'state, 'event ) mtrel # ('pred) tded)``);
@@ -83,7 +83,19 @@ Define  `
 ((composeMuRe Re1 Re2 (Sym,P,S1,S2) (e::ev) (Sym'',P'',S1'',S2'')) = 
  (∃Sym' P' S1' S2' rel1 rel2 Re1' Re2'. (composeRel rel1 rel2 (Sym,P,S1,S2) e (Sym',P',S1',S2')) ∧ (rel1 (Sym,(IMAGE OUTL P),S1) (OUTL e) (Sym',(IMAGE OUTL P'),S1')) ∧ (Re1 (Sym,(IMAGE OUTL P),S1) (MAP OUTL (e::ev)) (Sym'',(IMAGE OUTL P''),S1'')) ∧ (rel2 (Sym,(IMAGE OUTR P),S2) (OUTR e) (Sym',(IMAGE OUTR P'),S2')) ∧ (Re2 (Sym,(IMAGE OUTR P),S2) (MAP OUTR (e::ev)) (Sym'',(IMAGE OUTR P''),S2'')) ∧ (Re2' (Sym',(IMAGE OUTR P'),S2') (MAP OUTR ev) (Sym'',(IMAGE OUTR P''),S2'')) ∧ (Re1' (Sym',(IMAGE OUTL P'),S1') (MAP OUTL ev) (Sym'',(IMAGE OUTL P''),S1'')) ∧ (composeMuRe Re1' Re2' (Sym',P',S1',S2') ev (Sym'',P'',S1'',S2''))))
 `;*)
-
+val FIRST_def =
+Define  `
+        ((FIRST (a,b,c)) = a)
+        `;
+val SECOND_def =
+Define  `
+        ((SECOND (a,b,c)) = b)
+        `;
+val THIRD_def =
+Define  `
+        ((THIRD (a,b,c)) = c)
+        `;
+(*        
 val composeMuRe_def =
 Define  `
         ((composeMuRe Re1 Re2 (Sym,P,S1,S2) [] (Sym',P',S1',S2')) = ((Sym,P,S1,S2) = (Sym',P',S1',S2')))  ∧
@@ -98,12 +110,21 @@ Define  `
         ((composeMuRe Re1 Re2 (Sym,P,S1,S2) (e::ev) (Sym'',P'',S1'',S2'')) = 
          (∃Sym' P' S1' S2'. (composeMuRe Re1 Re2 (Sym,P,S1,S2) [e] (Sym',P',S1',S2')) ∧ (composeMuRe Re1 Re2 (Sym',P',S1',S2') ev (Sym'',P'',S1'',S2''))))
         `;
-
-
+*)
+val composeMuRe_def =
+Define  `
+        ((composeMuRe (Re1:(('event1 + 'eventS), 'pred1, 'state1, 'symb) mtrel) (Re2:(('event2 + 'eventS), 'pred2, 'state2, 'symb) mtrel) (Sym,P,S1,S2) []) = (Sym,P,S1,S2)) ∧
+((composeMuRe (Re1:(('event1 + 'eventS), 'pred1, 'state1, 'symb) mtrel) (Re2:(('event2 + 'eventS), 'pred2, 'state2, 'symb) mtrel) (Sym,P,S1,S2) ((INL (INL (E:'event1)))::ev))
+ = composeMuRe Re1 Re2 ((FIRST(Re1 (Sym,(IMAGE OUTL P),S1) [INL E]),((SECOND(Re1 (Sym,(IMAGE OUTL P),S1) [INL E]))<+>(IMAGE OUTR P)),THIRD(Re1 (Sym,(IMAGE OUTL P),S1) [INL E]),S2)) ev)   ∧
+((composeMuRe (Re1:(('event1 + 'eventS), 'pred1, 'state1, 'symb) mtrel) (Re2:(('event2 + 'eventS), 'pred2, 'state2, 'symb) mtrel) (Sym,P,S1,S2) ((INR (INL (E:'event2)))::ev))
+ = composeMuRe Re1 Re2 ((FIRST(Re2 (Sym,(IMAGE OUTR P),S2) [INL E]),((IMAGE OUTL P)<+>(SECOND(Re2 (Sym,(IMAGE OUTR P),S2) [INL E]))),S1,THIRD(Re2 (Sym,(IMAGE OUTR P),S2) [INL E]))) ev) ∧
+((composeMuRe (Re1:(('event1 + 'eventS), 'pred1, 'state1, 'symb) mtrel) (Re2:(('event2 + 'eventS), 'pred2, 'state2, 'symb) mtrel) (Sym,P,S1,S2) ((INR (INR (E:'eventS)))::ev))
+ = composeMuRe Re1 Re2 (((FIRST(Re1 (Sym,(IMAGE OUTL P),S1) [INR E]))∪(FIRST(Re2 (Sym,(IMAGE OUTR P),S2) [INR E])),((SECOND(Re1 (Sym,(IMAGE OUTL P),S1) [INR E]))<+>(SECOND(Re2 (Sym,(IMAGE OUTR P),S2) [INR E]))),THIRD(Re1 (Sym,(IMAGE OUTL P),S1) [INR E]),THIRD(Re2 (Sym,(IMAGE OUTR P),S2) [INR E]))) ev)
+`;
 val composeMuRe_empty_event_thm = store_thm(
   "composeMuRe_empty_event_thm", ``
-∀Re1 Re2 Sym P S1 S2 E Sym' P' S1' S2'.
-(composeMuRe Re1 Re2 (Sym,P,S1,S2) [] (Sym',P',S1',S2')) ⇔ ((Sym,P,S1,S2) = (Sym',P',S1',S2'))
+∀Re1 Re2 Sym P S1 S2.
+(composeMuRe Re1 Re2 (Sym,P,S1,S2) []) = (Sym,P,S1,S2)
                                        ``,
  FULL_SIMP_TAC std_ss [composeMuRe_def]  
   );
@@ -128,7 +149,7 @@ val composeMuRe_multi_events_thm = store_thm(
                                   Q.EXISTS_TAC `S1'³'` >> Q.EXISTS_TAC `S2'³'` >> Q.EXISTS_TAC `rel1` >> Q.EXISTS_TAC `rel2` >>
                                   Q.EXISTS_TAC `Re1'` >> Q.EXISTS_TAC `Re2'` >> REPEAT STRIP_TAC >> ASM_REWRITE_TAC[] >> ASM_REWRITE_TAC[]
                                                                                                                                         
-  );*)
+  );
 
 val composeMuRe_StatetoConfig_thm = store_thm(
   "composeMuRe_StatetoConfig_thm", ``
@@ -136,7 +157,7 @@ val composeMuRe_StatetoConfig_thm = store_thm(
 (composeMuRe Re1 Re2 (Sym,P,S1,S2) E (Sym',P',S1',S2')) ==> (∃Conf Conf'. (composeMuRe Re1 Re2 Conf E Conf') ∧ (Conf = (Sym,P,S1,S2)) ∧ (Conf' = (Sym',P',S1',S2')))
                                        ``,
  FULL_SIMP_TAC std_ss [composeMuRe_def]  
-  );
+  );*)
 
 
 (*
@@ -180,7 +201,7 @@ val (composeMuRe_rules, composeMuRe_ind, composeMuRe_cases)
    ((Evs = (e::ev)) ∧ (composeRel rel1 rel2 Conf e Conf') ∧ (Conf = (Sym,P,S1,S2)) ∧ (Conf' = (Sym',P',S1',S2')) ∧ (Conf'' = (Sym'',P'',S1'',S2'')) ∧ (rel1 (Sym,(IMAGE OUTL P),S1) (OUTL e) (Sym',(IMAGE OUTL P'),S1')) ∧ (Re1 (Sym,(IMAGE OUTL P),S1) (MAP OUTL Evs) (Sym'',(IMAGE OUTL P''),S1'')) ∧ (rel2 (Sym,(IMAGE OUTR P),S2) (OUTR e) (Sym',(IMAGE OUTR P'),S2')) ∧ (Re2 (Sym,(IMAGE OUTR P),S2) (MAP OUTR Evs) (Sym'',(IMAGE OUTR P''),S2'')) ∧ (Re2' (Sym',(IMAGE OUTR P'),S2') (MAP OUTR ev) (Sym'',(IMAGE OUTR P''),S2'')) ∧ (Re1' (Sym',(IMAGE OUTL P'),S1') (MAP OUTL ev) (Sym'',(IMAGE OUTL P''),S1'')) ∧ (composeMuRe Re1' Re2' Conf' ev Conf'')) ==> (composeMuRe Re1 Re2 Conf Evs Conf''))     
 `; 
 *)
-(* compose multi transition system *)
+(* compose multi transition system *)(*
 val _ = Parse.type_abbrev("MulComOpr", 
   ``:('symb, 'pred1, 'state1, 'event1 + 'eventS) multransys ->
   ('symb, 'pred2, 'state2, 'event2 + 'eventS) multransys -> 
@@ -197,10 +218,23 @@ val _ = set_mapped_fixity { fixity = Infixl 95,
 
 val _ = overload_on ("apply_composeMultiOperation", ``composeMultiOperation``);
 
- (*                                   
-val composeMultiOperation_def =
+ val composeMultiOperation_def =
 Define`
       (composeMultiOperation ((rel1:(('event1 + 'eventS), 'pred1, 'state1, 'symb) mtrel),(ded1:('pred1) tded)) ((rel2:(('event2 + 'eventS), 'pred2, 'state2, 'symb) mtrel),(ded2:('pred2) tded)) =
                              ((λ(Sym,P,S1,S2) E (Sym',P',S1',S2'). composeMuRe rel1 rel2 (Sym,P,S1,S2) E (Sym',P',S1',S2')), composeDed ded1 ded2): ('symb, 'pred1 + 'pred2, 'state1 # 'state2, (('event1+'eventS) + ('event2 +'eventS))) multransys)
       `;*)
+
+val combinelists_def =
+Define`
+      (combinelists ([]:α list) ([]:β list) = (APPEND [] [])) ∧
+(combinelists ([]:α list) ((e2::ev2):β list) = APPEND (APPEND [] [INR e2]) (combinelists [] ev2))  ∧
+(combinelists ((e1::ev1):α list) ([]:β list) = APPEND (APPEND [INL e1] []) (combinelists ev1 [])) ∧
+(combinelists ((e1::ev1):α list) ((e2::ev2):β list) = APPEND (APPEND [INL e1] [INR e2]) (combinelists ev1 ev2))
+`;      
+
+ val composeMultiOperation_def =
+Define`
+      composeMultiOperation Re1 (Sym1,P1,S1) E1 Re2 (Sym2,P2,S2) E2 = (composeMuRe Re1 Re2 ((Sym1∪Sym2),(P1<+>P2),S1,S2) (combinelists E1 E2))
+      `;
 val _ = export_theory();
+
